Splinter/Program.i.dfy
@@ -60,32 +60,91 @@ module ProgramMachineMod {
     false
   }
 
-  predicate Query(s: Variables, s': Variables, k: Key, v: Value)
+  predicate Query(s: Variables, s': Variables, k: Key, v: Value, sk: BetreeMachineMod.Skolem)
   {
     && s.WF()
     && s'.journal == s.journal
-    && BetreeMachineMod.Query(s.betree, s'.betree, k, v)
+    && BetreeMachineMod.Query(s.betree, s'.betree, s.cache, k, v, sk)
+    && s'.cache == s.cache  // no cache writes
   }
 
-  predicate Put(s: Variables, s': Variables, k: Key, v: Value)
+  predicate Put(s: Variables, s': Variables, k: Key, v: Value, sk: BetreeMachineMod.Skolem)
   {
     && s.WF()
     && JournalMachineMod.Append(s.journal, s'.journal, MessagePut(k, v))
-    && BetreeMachineMod.Put(s.betree, s'.betree, k, v)
+    && BetreeMachineMod.Put(s.betree, s'.betree, k, v, sk)
+    && s'.cache == s.cache  // no cache writes
   }
 
-  predicate JournalInternal(s: Variables, s': Variables)
+  // TODO move to Sets.i
+  predicate SetsMutuallyDisjoint<T>(sets: seq<set<T>>) {
+    forall i, j | 0<=i<|sets| && 0<=j<|sets| && i!=j :: sets[i] !! sets[j]
+  }
+
+  predicate AllocsDisjoint(s: Variables)
+  {
+    SetsMutuallyDisjoint([
+      {SUPERBLOCK_ADDRESS().au},
+      JournalMachineMod.Alloc(s.journal),
+      BetreeMachineMod.Alloc(s.betree)
+      ])
+  }
+
+  predicate WritesOkay(cacheOps: CacheIfc.Ops, alloc: set<AU>)
+  {
+    forall op | op in cacheOps :: op.cu.au in alloc
+  }
+  
+  // How do the subsystems negotiate for more alloc?
+  // They're always free to write into their existing alloc -- Journal is going to want
+  // to do that all the time, maintaining its own internal allocation tracker, to avoid
+  // writing out new allocation bitmap summaries. In principle, Journal can ask to grow
+  // its alloc.
+  // Betree, on the other hand: it's gonna alloc all the darn time. We need to make
+  // sure that when it does, the new AUs are disjoint with our alloc (the superblocks)
+  // and the Journal's existing alloc.
+  // So how do we record each system's current alloc?
+  // Do subsystems "know" their current alloc? I guess they do, ghostily --
+  // when BeTree.B+tree links a new AU into an in-progress B+tree, it claims another AU,
+  // and updates its ghost alloc -- oh, that's just a function over all reachable state on
+  // disk!
+  // At sb time, that's the alloc it publishes to a marshalled alloc record on the disk.
+  // (Do we need to do that here, if the physical thing isn't gonna do that? Hrm.)
+  // So at Journal-alloc time, we just test against the betree's ghost alloc?
+  //
+  // The real system would have ghost views of subsystem allocs, a single physical alloc bitmap,
+  // and an invariant that the physical alloc bitmap is the union of the ghosty ones.
+  // NO that's not right! They need separate allocs so they can record them precisely (and
+  // separately, since they update out of sync), so that crashes correctly reflect what has
+  // changed.
+  // Well, maybe they don't need to be recorded separately. Maybe it's okay if the sb always
+  // points to a single alloc that's an precise union of the underlying subsystems.
+  // When journal wants to grow, it allocates AU from the central allocator.
+  // When Betree wants to grow, it allocates AU from the central allocator.
+  // These only affect in-memory state.
+  // When sb commits, it includes the state of ... uh oh, which betree? Ephemeral or frozen?
+  // so I guess we need to track them separately, so that we can record the frozen's allocation
+  // to the sb, while still tracking the ephemeral alloc in memory (for next freeze).
+  // At that point we COULD write frozen-alloc UNION journal-alloc to the sb, but is that
+  // a false economy? I guess not -- we have to coordinate across subsystems, and they share
+  // an invariant that makes them reduntant anyway. Hrmm.
+
+  predicate JournalInternal(s: Variables, s': Variables, cacheOps: CacheIfc.Ops, sk: JournalMachineMod.Skolem)
   {
     && s.WF()
-    && JournalMachineMod.Internal(s.journal, s'.journal)
+    && JournalMachineMod.Internal(s.journal, s'.journal, s.cache, cacheOps, sk)
     && s'.betree == s.betree
+    && CacheIfc.ApplyWrites(s.cache, s'.cache, cacheOps)
+    && WritesOkay(cacheOps, JournalMachineMod.Alloc(s'.journal))
+    && AllocsDisjoint(s')
   }
 
-  predicate BetreeInternal(s: Variables, s': Variables)
+  predicate BetreeInternal(s: Variables, s': Variables, cacheOps: CacheIfc.Ops, sk: BetreeMachineMod.Skolem)
   {
     && s.WF()
     && s'.journal == s.journal
-    && BetreeMachineMod.Internal(s.betree, s'.betree)
+    && BetreeMachineMod.Internal(s.betree, s'.betree, s.cache, cacheOps, sk)
+    && CacheIfc.ApplyWrites(s.cache, s'.cache, cacheOps)
   }
 
   predicate ReqSync(s: Variables, s': Variables, syncReqId: SyncReqId)
@@ -137,35 +196,32 @@ module ProgramMachineMod {
 
   datatype Step =
     | RecoverStep()
-    | QueryStep(k: Key, v: Value)
-    | PutStep(k: Key, v: Value)
-    | JournalInternalStep()
-    | BetreeInternalStep()
+    | QueryStep(k: Key, v: Value, bsk: BetreeMachineMod.Skolem)
+    | PutStep(k: Key, v: Value, bsk: BetreeMachineMod.Skolem)
+    | JournalInternalStep(jsk: JournalMachineMod.Skolem)
+    | BetreeInternalStep(BetreeMachineMod.Skolem)
     | ReqSyncStep(syncReqId: SyncReqId)
     | CompleteSyncStep(syncReqId: SyncReqId)
     | CommitStartStep(seqBoundary: LSN)
     | CommitCompleteStep()
     
-  predicate NextStep(s: Variables, s': Variables, step: Step) {
-    && cacheOps.writeSet !! IReads(s.betree)  // We only wrote fresh or existing stuff
-    && IReads(s'.journal) == IReads(s.journal) + cacheOps.writeSet  // goes down in the journal
-//    && IReads(s'.journal) !! IReads(s'.betree)  // Layer below needs to enforce framing disjointness
+  predicate NextStep(s: Variables, s': Variables, cacheOps: CacheIfc.Ops, step: Step) {
     && match step {
       case RecoverStep() => Recover(s, s')
-      case QueryStep(k: Key, v: Value) => Query(s, s', k, v)
-      case PutStep(k: Key, v: Value) => Put(s, s', k, v)
-      case JournalInternalStep() => JournalInternal(s, s', cacheOps)
-      case BetreeInternalStep() => BetreeInternal(s, s')
-      case ReqSyncStep(syncReqId: SyncReqId) => ReqSync(s, s', syncReqId)
-      case CompleteSyncStep(syncReqId: SyncReqId) => CompleteSync(s, s', syncReqId)
-      case CommitStartStep(seqBoundary: LSN) => CommitStart(s, s', seqBoundary)
+      case QueryStep(k, v, sk) => Query(s, s', k, v, sk)
+      case PutStep(k, v, sk) => Put(s, s', k, v, sk)
+      case JournalInternalStep(sk) => JournalInternal(s, s', cacheOps, sk)
+      case BetreeInternalStep(sk) => BetreeInternal(s, s', cacheOps, sk)
+      case ReqSyncStep(syncReqId) => ReqSync(s, s', syncReqId)
+      case CompleteSyncStep(syncReqId) => CompleteSync(s, s', syncReqId)
+      case CommitStartStep(seqBoundary) => CommitStart(s, s', seqBoundary)
       case CommitCompleteStep() => CommitComplete(s, s')
     }
   }
 
   predicate Next(s: Variables, s': Variables) {
-    exists step ::
-      && NextStep(s, s', step)
+    exists cacheOps,step ::
+      && NextStep(s, s', cacheOps, step)
       //&& AllocationTableMachineMod.Disjoint(s'.journal.allocation, s'.betree.allocation)
   }
 }
@@ -206,6 +262,13 @@ module ProgramInterpMod {
     [ SUPERBLOCK_ADDRESS().au ]
   }
  
+  // Program will have a runtime view of what (ghost) alloc each subsystem thinks it's using,
+  // and use that to filter the dvs here.
+  // Those ghost views will invariantly match the IReads functions of the actual disk -- that is,
+  // * if we were to recover after a crash (when the physical alloc is empty), we'd fault in
+  // an alloc table for the subsystem.
+  // * that alloc table would invariantly match IReads.
+  //
   // IM == Interpret as InterpMod
   // Oh man we're gonna have a family of IReads predicates that capture the
   // heapiness of DiskView, aren't we?
